localize error

src/Init/Data/Array/Lex/Basic.lean
@@ -6,12 +6,9 @@ Author: Kim Morrison
 module
 
 prelude
-public import Init.Core
-import Init.Data.Array.Basic
-import Init.Data.Nat.Lemmas
-import Init.Data.Range.Polymorphic.Iterators
-import Init.Data.Range.Polymorphic.Nat
-import Init.Data.Iterators.Consumers
+public import Init.Data.Array.Basic
+public import Init.Data.Nat.Lemmas
+public import Init.Data.Range
 
 public section
 
@@ -29,9 +26,9 @@ Specifically, `Array.lex as bs lt` is true if
 * there is an index `i` such that `lt as[i] bs[i]`, and for all `j < i`, `as[j] == bs[j]`.
 -/
 def lex [BEq α] (as bs : Array α) (lt : α → α → Bool := by exact (· < ·)) : Bool := Id.run do
-  for h : i in 0...(min as.size bs.size) do
-    -- TODO: `get_elem_tactic` should be able to find this itself.
-    have : i < min as.size bs.size := Std.PRange.lt_upper_of_mem h
+  for h : i in [0 : min as.size bs.size] do
+    -- TODO: `omega` should be able to find this itself.
+    have : i < min as.size bs.size := Membership.get_elem_helper h rfl
     if lt as[i] bs[i] then
       return true
     else if as[i] != bs[i] then
